Proof.lean
@@ -1,0 +1,11 @@
+import Proof.Syntax
+import Proof.Semantics
+import Proof.Stack
+import Proof.Analysis
+import Proof.CorrectnessRelation
+import Proof.REInv
+import Proof.AccessImpliesDep
+import Proof.StackDepChain
+import Proof.PartialOnStack
+import Proof.AbstractDetectsCycle
+import Proof.Algorithm
